HS_ODEs.thy
@@ -98,30 +98,30 @@ no_notation g_orbit ("\<gamma>")
 
 subsection \<open> Differential Invariants \<close>
 
-definition diff_invariant :: "('a \<Rightarrow> bool) \<Rightarrow> (real \<Rightarrow> ('a::real_normed_vector) \<Rightarrow> 'a) \<Rightarrow> 
+definition diff_inv :: "('a \<Rightarrow> bool) \<Rightarrow> (real \<Rightarrow> ('a::real_normed_vector) \<Rightarrow> 'a) \<Rightarrow> 
   ('a \<Rightarrow> real set) \<Rightarrow> 'a set \<Rightarrow> real \<Rightarrow> ('a \<Rightarrow> bool) \<Rightarrow> bool" 
-  where "diff_invariant I f U S t\<^sub>0 G \<equiv> (\<Union> \<circ> (\<P> (g_orbital f G U S t\<^sub>0))) {s. I s} \<subseteq> {s. I s}"
+  where "diff_inv I f U S t\<^sub>0 G \<equiv> (\<Union> \<circ> (\<P> (g_orbital f G U S t\<^sub>0))) {s. I s} \<subseteq> {s. I s}"
 
-lemma diff_invariant_eq: "diff_invariant I f U S t\<^sub>0 G = 
+lemma diff_inv_eq: "diff_inv I f U S t\<^sub>0 G = 
   (\<forall>s. I s \<longrightarrow> (\<forall>X\<in>Sols U S f t\<^sub>0 s. (\<forall>t\<in>U s.(\<forall>\<tau>\<in>(down (U s) t). G (X \<tau>)) \<longrightarrow> I (X t))))"
-  unfolding diff_invariant_def g_orbital_eq image_le_pred by auto
+  unfolding diff_inv_def g_orbital_eq image_le_pred by auto
 
 lemma diff_inv_eq_inv_set:
-  "diff_invariant I f U S t\<^sub>0 G = (\<forall>s. I s \<longrightarrow> (g_orbital f G U S t\<^sub>0 s) \<subseteq> {s. I s})"
-  unfolding diff_invariant_eq g_orbital_eq image_le_pred by auto
+  "diff_inv I f U S t\<^sub>0 G = (\<forall>s. I s \<longrightarrow> (g_orbital f G U S t\<^sub>0 s) \<subseteq> {s. I s})"
+  unfolding diff_inv_eq g_orbital_eq image_le_pred by auto
 
-lemma "diff_invariant I f U S t\<^sub>0 (\<lambda>s. True) \<Longrightarrow> diff_invariant I f U S t\<^sub>0 G"
-  unfolding diff_invariant_eq by auto
+lemma "diff_inv I f U S t\<^sub>0 (\<lambda>s. True) \<Longrightarrow> diff_inv I f U S t\<^sub>0 G"
+  unfolding diff_inv_eq by auto
 
-named_theorems diff_invariant_rules "rules for certifying differential invariants"
+named_theorems diff_inv_rules "rules for certifying differential invariants"
 
-lemma diff_invariant_eq_rule [diff_invariant_rules]:
+lemma diff_inv_eq_rule [diff_inv_rules]:
   fixes \<mu>::"'a::banach \<Rightarrow> real"
   assumes Uhyp: "\<And>s. s \<in> S \<Longrightarrow> is_interval (U s)"
     and dX: "\<And>X t. (D X = (\<lambda>\<tau>. f \<tau> (X \<tau>)) on U(X t\<^sub>0)) \<Longrightarrow> 
   \<forall>\<tau>\<in>(down (U(X t\<^sub>0)) t). G (X \<tau>) \<Longrightarrow> D (\<lambda>\<tau>. \<mu> (X \<tau>) - \<nu> (X \<tau>)) = (\<lambda>\<tau>. \<tau> *\<^sub>R 0) on U(X t\<^sub>0)"
-  shows "diff_invariant (\<lambda>s. \<mu> s = \<nu> s) f U S t\<^sub>0 G"
-proof(simp add: diff_invariant_eq ivp_sols_def, clarsimp)
+  shows "diff_inv (\<lambda>s. \<mu> s = \<nu> s) f U S t\<^sub>0 G"
+proof(simp add: diff_inv_eq ivp_sols_def, clarsimp)
   fix X t 
   assume xivp:"D X = (\<lambda>\<tau>. f \<tau> (X \<tau>)) on U (X t\<^sub>0)" "\<mu> (X t\<^sub>0) = \<nu> (X t\<^sub>0)" "X \<in> U (X t\<^sub>0) \<rightarrow> S"
     and tHyp:"t \<in> U (X t\<^sub>0)" and t0Hyp: "t\<^sub>0 \<in> U (X t\<^sub>0)" 
@@ -137,22 +137,22 @@ proof(simp add: diff_invariant_eq ivp_sols_def, clarsimp)
     by (simp add: xivp(2))
 qed
 
-lemma diff_invariant_eq_rule_old:
+lemma diff_inv_eq_rule_old:
   fixes \<mu>::"'a::banach \<Rightarrow> real"
   assumes Uhyp: "\<And>s. s \<in> S \<Longrightarrow> is_interval (U s)"
     and dX: "\<And>X. (D X = (\<lambda>\<tau>. f \<tau> (X \<tau>)) on U(X t\<^sub>0)) \<Longrightarrow> (D (\<lambda>\<tau>. \<mu>(X \<tau>)-\<nu>(X \<tau>)) = ((*\<^sub>R) 0) on U(X t\<^sub>0))"
-  shows "diff_invariant (\<lambda>s. \<mu> s = \<nu> s) f U S t\<^sub>0 G"
-  apply(rule diff_invariant_eq_rule[OF Uhyp], simp)
+  shows "diff_inv (\<lambda>s. \<mu> s = \<nu> s) f U S t\<^sub>0 G"
+  apply(rule diff_inv_eq_rule[OF Uhyp], simp)
   by (frule dX, simp)
 
-lemma diff_invariant_leq_rule [diff_invariant_rules]:
+lemma diff_inv_leq_rule [diff_inv_rules]:
   fixes \<mu>::"'a::banach \<Rightarrow> real"
   assumes Uhyp: "\<And>s. s \<in> S \<Longrightarrow> is_interval (U s)"
     and Gg: "\<And>X. (D X = (\<lambda>\<tau>. f \<tau> (X \<tau>)) on U(X t\<^sub>0)) \<Longrightarrow> (\<forall>\<tau>\<in>U(X t\<^sub>0). \<tau> > t\<^sub>0 \<longrightarrow> G (X \<tau>) \<longrightarrow> \<mu>' (X \<tau>) \<ge> \<nu>' (X \<tau>))"
     and Gl: "\<And>X. (D X = (\<lambda>\<tau>. f \<tau> (X \<tau>)) on U(X t\<^sub>0)) \<Longrightarrow> (\<forall>\<tau>\<in>U(X t\<^sub>0). \<tau> < t\<^sub>0 \<longrightarrow> \<mu>' (X \<tau>) \<le> \<nu>' (X \<tau>))"
     and dX: "\<And>X. (D X = (\<lambda>\<tau>. f \<tau> (X \<tau>)) on U(X t\<^sub>0)) \<Longrightarrow> D (\<lambda>\<tau>. \<mu>(X \<tau>)-\<nu>(X \<tau>)) = (\<lambda>\<tau>. \<mu>'(X \<tau>)-\<nu>'(X \<tau>)) on U(X t\<^sub>0)"
-  shows "diff_invariant (\<lambda>s. \<nu> s \<le> \<mu> s) f U S t\<^sub>0 G"
-proof(simp_all add: diff_invariant_eq ivp_sols_def, safe)
+  shows "diff_inv (\<lambda>s. \<nu> s \<le> \<mu> s) f U S t\<^sub>0 G"
+proof(simp_all add: diff_inv_eq ivp_sols_def, safe)
   fix X t assume Ghyp: "\<forall>\<tau>. \<tau> \<in> U (X t\<^sub>0) \<and> \<tau> \<le> t \<longrightarrow> G (X \<tau>)"
   assume xivp: "D X = (\<lambda>x. f x (X x)) on U (X t\<^sub>0)" "\<nu> (X t\<^sub>0) \<le> \<mu> (X t\<^sub>0)" "X \<in> U (X t\<^sub>0) \<rightarrow> S"
   assume tHyp: "t \<in> U (X t\<^sub>0)" and t0Hyp: "t\<^sub>0 \<in> U (X t\<^sub>0)" 
@@ -185,14 +185,14 @@ proof(simp_all add: diff_invariant_eq ivp_sols_def, safe)
     using xivp by blast
 qed
 
-lemma diff_invariant_less_rule [diff_invariant_rules]:
+lemma diff_inv_less_rule [diff_inv_rules]:
   fixes \<mu>::"'a::banach \<Rightarrow> real"
   assumes Uhyp: "\<And>s. s \<in> S \<Longrightarrow> is_interval (U s)"
     and Gg: "\<And>X. (D X = (\<lambda>\<tau>. f \<tau> (X \<tau>)) on U(X t\<^sub>0)) \<Longrightarrow> (\<forall>\<tau>\<in>U(X t\<^sub>0). \<tau> > t\<^sub>0 \<longrightarrow> G (X \<tau>) \<longrightarrow> \<mu>' (X \<tau>) \<ge> \<nu>' (X \<tau>))"
     and Gl: "\<And>X. (D X = (\<lambda>\<tau>. f \<tau> (X \<tau>)) on U(X t\<^sub>0)) \<Longrightarrow> (\<forall>\<tau>\<in>U(X t\<^sub>0). \<tau> < t\<^sub>0 \<longrightarrow> \<mu>' (X \<tau>) \<le> \<nu>' (X \<tau>))"
     and dX: "\<And>X. (D X = (\<lambda>\<tau>. f \<tau> (X \<tau>)) on U(X t\<^sub>0)) \<Longrightarrow> D (\<lambda>\<tau>. \<mu>(X \<tau>)-\<nu>(X \<tau>)) = (\<lambda>\<tau>. \<mu>'(X \<tau>)-\<nu>'(X \<tau>)) on U(X t\<^sub>0)"
-  shows "diff_invariant (\<lambda>s. \<nu> s < \<mu> s) f U S t\<^sub>0 G"
-proof(simp_all add: diff_invariant_eq ivp_sols_def, safe)
+  shows "diff_inv (\<lambda>s. \<nu> s < \<mu> s) f U S t\<^sub>0 G"
+proof(simp_all add: diff_inv_eq ivp_sols_def, safe)
   fix X t assume Ghyp: "\<forall>\<tau>. \<tau> \<in> U (X t\<^sub>0) \<and> \<tau> \<le> t \<longrightarrow> G (X \<tau>)"
   assume xivp: "D X = (\<lambda>x. f x (X x)) on U (X t\<^sub>0)" "\<nu> (X t\<^sub>0) < \<mu> (X t\<^sub>0)" "X \<in> U (X t\<^sub>0) \<rightarrow> S"
   assume tHyp: "t \<in> U (X t\<^sub>0)" and t0Hyp: "t\<^sub>0 \<in> U (X t\<^sub>0)" 
@@ -225,46 +225,46 @@ proof(simp_all add: diff_invariant_eq ivp_sols_def, safe)
     using xivp by blast
 qed
 
-lemma diff_invariant_nleq_rule:
+lemma diff_inv_nleq_rule:
   fixes \<mu>::"'a::banach \<Rightarrow> real"
-  shows "diff_invariant (\<lambda>s. \<not> \<nu> s \<le> \<mu> s) f U S t\<^sub>0 G \<longleftrightarrow> diff_invariant (\<lambda>s. \<nu> s > \<mu> s) f U S t\<^sub>0 G"
-  unfolding diff_invariant_eq apply safe
+  shows "diff_inv (\<lambda>s. \<not> \<nu> s \<le> \<mu> s) f U S t\<^sub>0 G \<longleftrightarrow> diff_inv (\<lambda>s. \<nu> s > \<mu> s) f U S t\<^sub>0 G"
+  unfolding diff_inv_eq apply safe
   by (clarsimp, erule_tac x=s in allE, simp, erule_tac x=X in ballE, force, force)+
 
-lemma diff_invariant_neq_rule [diff_invariant_rules]:
+lemma diff_inv_neq_rule [diff_inv_rules]:
   fixes \<mu>::"'a::banach \<Rightarrow> real"
-  assumes "diff_invariant (\<lambda>s. \<nu> s < \<mu> s) f U S t\<^sub>0 G"
-    and "diff_invariant (\<lambda>s. \<nu> s > \<mu> s) f U S t\<^sub>0 G"
-  shows "diff_invariant (\<lambda>s. \<nu> s \<noteq> \<mu> s) f U S t\<^sub>0 G"
-proof(unfold diff_invariant_eq, clarsimp)
+  assumes "diff_inv (\<lambda>s. \<nu> s < \<mu> s) f U S t\<^sub>0 G"
+    and "diff_inv (\<lambda>s. \<nu> s > \<mu> s) f U S t\<^sub>0 G"
+  shows "diff_inv (\<lambda>s. \<nu> s \<noteq> \<mu> s) f U S t\<^sub>0 G"
+proof(unfold diff_inv_eq, clarsimp)
   fix s::'a and X::"real \<Rightarrow> 'a" and t::real
   assume "\<nu> s \<noteq> \<mu> s" and Xhyp: "X \<in> Sols U S f t\<^sub>0 s" 
      and thyp: "t \<in> U s" and Ghyp: "\<forall>\<tau>. \<tau> \<in> U s \<and> \<tau> \<le> t \<longrightarrow> G (X \<tau>)"
   hence "\<nu> s < \<mu> s \<or> \<nu> s > \<mu> s"
     by linarith
   moreover have "\<nu> s < \<mu> s \<Longrightarrow> \<nu> (X t) < \<mu> (X t)"
-    using assms(1) Xhyp thyp Ghyp unfolding diff_invariant_eq by auto
+    using assms(1) Xhyp thyp Ghyp unfolding diff_inv_eq by auto
   moreover have "\<nu> s > \<mu> s \<Longrightarrow> \<nu> (X t) > \<mu> (X t)"
-    using assms(2) Xhyp thyp Ghyp unfolding diff_invariant_eq by auto
+    using assms(2) Xhyp thyp Ghyp unfolding diff_inv_eq by auto
   ultimately show "\<nu> (X t) = \<mu> (X t) \<Longrightarrow> False"
     by auto
 qed
 
-lemma diff_invariant_neq_rule_converse:
+lemma diff_inv_neq_rule_converse:
   fixes \<mu>::"'a::banach \<Rightarrow> real"
   assumes Uhyp: "\<And>s. s \<in> S \<Longrightarrow> is_interval (U s)" "\<And>s t. s \<in> S \<Longrightarrow> t \<in> U s \<Longrightarrow> t\<^sub>0 \<le> t"
     and conts: "\<And>X. (D X = (\<lambda>\<tau>. f \<tau> (X \<tau>)) on U(X t\<^sub>0)) \<Longrightarrow> continuous_on (\<P> X (U (X t\<^sub>0))) \<nu>"
       "\<And>X. (D X = (\<lambda>\<tau>. f \<tau> (X \<tau>)) on U(X t\<^sub>0)) \<Longrightarrow> continuous_on (\<P> X (U (X t\<^sub>0))) \<mu>"
-    and dI:"diff_invariant (\<lambda>s. \<nu> s \<noteq> \<mu> s) f U S t\<^sub>0 G"
-  shows "diff_invariant (\<lambda>s. \<nu> s < \<mu> s) f U S t\<^sub>0 G"
-proof(unfold diff_invariant_eq ivp_sols_def, clarsimp)
+    and dI:"diff_inv (\<lambda>s. \<nu> s \<noteq> \<mu> s) f U S t\<^sub>0 G"
+  shows "diff_inv (\<lambda>s. \<nu> s < \<mu> s) f U S t\<^sub>0 G"
+proof(unfold diff_inv_eq ivp_sols_def, clarsimp)
   fix X t assume Ghyp: "\<forall>\<tau>. \<tau> \<in> U (X t\<^sub>0) \<and> \<tau> \<le> t \<longrightarrow> G (X \<tau>)"
   assume xivp: "D X = (\<lambda>x. f x (X x)) on U (X t\<^sub>0)" "\<nu> (X t\<^sub>0) < \<mu> (X t\<^sub>0)" "X \<in> U (X t\<^sub>0) \<rightarrow> S"
   assume tHyp: "t \<in> U (X t\<^sub>0)" and t0Hyp: "t\<^sub>0 \<in> U (X t\<^sub>0)"
   hence "t\<^sub>0 \<le> t" and "\<mu> (X t) \<noteq> \<nu> (X t)"
     using xivp(3) Uhyp(2) apply force
     using dI tHyp xivp(2) Ghyp ivp_solsI[of X f U "X t\<^sub>0", OF xivp(1) _ xivp(3) t0Hyp]
-    unfolding diff_invariant_eq by force
+    unfolding diff_inv_eq by force
   moreover
   {assume ineq2:"\<nu> (X t) > \<mu> (X t)"
     note continuous_on_compose[OF vderiv_on_continuous_on[OF xivp(1)]]
@@ -282,24 +282,24 @@ proof(unfold diff_invariant_eq ivp_sols_def, clarsimp)
       by (auto simp: closed_segment_eq_real_ivl)
     hence "\<mu> (X \<tau>) \<noteq> \<nu> (X \<tau>)"
       using dI tHyp xivp(2) ivp_solsI[of X f U "X t\<^sub>0", OF xivp(1) _ xivp(3) t0Hyp]
-      unfolding diff_invariant_eq by force
+      unfolding diff_inv_eq by force
     hence "False"
       using \<open>\<mu> (X \<tau>) = \<nu> (X \<tau>)\<close> by blast}
   ultimately show "\<nu> (X t) < \<mu> (X t)"
     by fastforce
 qed
 
-lemma diff_invariant_conj_rule [diff_invariant_rules]:
-  assumes "diff_invariant I\<^sub>1 f U S t\<^sub>0 G"
-    and "diff_invariant I\<^sub>2 f U S t\<^sub>0 G"
-  shows "diff_invariant (\<lambda>s. I\<^sub>1 s \<and> I\<^sub>2 s) f U S t\<^sub>0 G"
-  using assms unfolding diff_invariant_def by auto
+lemma diff_inv_conj_rule [diff_inv_rules]:
+  assumes "diff_inv I\<^sub>1 f U S t\<^sub>0 G"
+    and "diff_inv I\<^sub>2 f U S t\<^sub>0 G"
+  shows "diff_inv (\<lambda>s. I\<^sub>1 s \<and> I\<^sub>2 s) f U S t\<^sub>0 G"
+  using assms unfolding diff_inv_def by auto
 
-lemma diff_invariant_disj_rule [diff_invariant_rules]:
-  assumes "diff_invariant I\<^sub>1 f U S t\<^sub>0 G"
-    and "diff_invariant I\<^sub>2 f U S t\<^sub>0 G"
-  shows "diff_invariant (\<lambda>s. I\<^sub>1 s \<or> I\<^sub>2 s) f U S t\<^sub>0 G"
-  using assms unfolding diff_invariant_def by auto
+lemma diff_inv_disj_rule [diff_inv_rules]:
+  assumes "diff_inv I\<^sub>1 f U S t\<^sub>0 G"
+    and "diff_inv I\<^sub>2 f U S t\<^sub>0 G"
+  shows "diff_inv (\<lambda>s. I\<^sub>1 s \<or> I\<^sub>2 s) f U S t\<^sub>0 G"
+  using assms unfolding diff_inv_def by auto
 
 subsection \<open> Picard-Lindeloef \<close>
 
